completed Sender class

main.dfy
@@ -6,30 +6,36 @@ class Sender {
   var name: string
   var balance: int
 
-  constructor(name: string)
-  {
+  constructor() {}
+
+  constructor FromName(name: string) {
     this.name := name;
     this.balance := 0;
   }
 
   method transfer(person: Sender, amount: int)
-  modifies this
-  modifies person
-  requires 0 < amount <= this.balance
+    modifies this, person
+    requires 0 < amount <= this.balance
   {
     this.balance := this.balance - amount;
     person.balance := person.balance + amount;
+  }
+
+  predicate equals(person: Sender)
+    reads this, person
+  {
+    this.name == person.name
   }
 }
 
 class Contract {
   var name: string
-  var operator: string
+  var operator: Sender
   var state: State
   var guess: Coin
   var pot: int
   var bet: int
-  var player: string
+  var player: Sender
   var hashedNumber: int
 
   ghost method transfer(amount : int, sender: string)
@@ -41,73 +47,75 @@ class Contract {
   }
 
 
-  constructor(sender: string, guess: Coin) {
+  constructor(sender: Sender, guess: Coin)
+  {
     this.operator := sender;
     this.guess := guess;
     this.state := IDLE;
     this.pot := 0;
     this.bet := 0;
-  }
+    this.player := new Sender();
+    }
 
-  method addToPot(amount: int, sender: string)
+  method addToPot(amount: int, sender: Sender)
     requires amount > 0
     modifies this
-    requires this.operator == sender
+    requires this.operator.equals(sender) == true
   {
     this.pot := this.pot + amount;
   }
 
-  method removeFromPot(amount: int, sender: string)
-    modifies this
-    requires this.state != BET_PLACED
-    requires this.operator == sender
-    requires amount > 0
-  {
-    this.transfer(amount,operator);
-    this.pot := pot - amount;
-  }
+  // method removeFromPot(amount: int, sender: string)
+  //   modifies this
+  //   requires this.state != BET_PLACED
+  //   requires this.operator == sender
+  //   requires amount > 0
+  // {
+  //   this.transfer(amount,operator);
+  //   this.pot := pot - amount;
+  // }
 
 
-  method createGame(sender: string, hashedNumber: int)
-    requires this.state == IDLE
-    requires this.operator == sender
-    modifies this
-  {
-    this.hashedNumber := hashedNumber;
-    this.state := GAME_AVAILABLE;
-  }
+  // method createGame(sender: string, hashedNumber: int)
+  //   requires this.state == IDLE
+  //   requires this.operator == sender
+  //   modifies this
+  // {
+  //   this.hashedNumber := hashedNumber;
+  //   this.state := GAME_AVAILABLE;
+  // }
 
-  method placeBet(guess : Coin, sender: string, amount: int)
-    requires state == GAME_AVAILABLE
-    requires sender != this.operator
-    requires 0 < amount <= this.pot
-    modifies this
-  {
-    this.state := BET_PLACED;
-    this.player := sender;
+  // method placeBet(guess : Coin, sender: string, amount: int)
+  //   requires state == GAME_AVAILABLE
+  //   requires sender != this.operator
+  //   requires 0 < amount <= this.pot
+  //   modifies this
+  // {
+  //   this.state := BET_PLACED;
+  //   this.player := sender;
 
-    this.bet := amount;
-    this.guess := guess;
-  }
+  //   this.bet := amount;
+  //   this.guess := guess;
+  // }
 
-  method decideBet(sender: string, secretNumber: int)
-    requires this.state == BET_PLACED
-    requires this.operator == sender
-    requires this.cryptohash(secretNumber) == this.hashedNumber
-    modifies this
-  {
-    var secret: Coin := getCoinFromGuess((secretNumber % 2) == 0);
-    if secret == this.guess {
-      // Player wins
-      this.pot := this.pot - this.bet;
-      this.transfer(2 * this.bet, this.player);
-    } else {
-      // Operator wins
-      this.pot := this.pot + this.bet;
-    }
-    this.bet := 0;
-    this.state := IDLE;
-  }
+  // method decideBet(sender: string, secretNumber: int)
+  //   requires this.state == BET_PLACED
+  //   requires this.operator == sender
+  //   requires this.cryptohash(secretNumber) == this.hashedNumber
+  //   modifies this
+  // {
+  //   var secret: Coin := getCoinFromGuess((secretNumber % 2) == 0);
+  //   if secret == this.guess {
+  //     // Player wins
+  //     this.pot := this.pot - this.bet;
+  //     this.transfer(2 * this.bet, this.player);
+  //   } else {
+  //     // Operator wins
+  //     this.pot := this.pot + this.bet;
+  //   }
+  //   this.bet := 0;
+  //   this.state := IDLE;
+  // }
 
 }
 
